add long_id.oeuf and id_nat.oeuf

shim.c
@@ -1,24 +1,26 @@
 #include "shim.h"
 // union nat* add(union nat* a, union nat* b);
 
-extern void* _$8(void*, void*);
-extern void* _$14(void*, void*);
+extern void* _$5(void*, void*);
+
+void* _$6(int size) {
+    return malloc(size);
+}
 
 int main() {
+    union nat* n = make_nat(3);
+
+    void* id = _$5(NULL, NULL);
+    void* m = VCALL(id, n);
+    printf("id(%d) = %d\n", read_nat(n), read_nat(m));
+
     /*
-    union nat* one = make_nat(1);
-    union nat* two = make_nat(2);
-
-    void* add = _$8(NULL, NULL);
-    void* sum = VCALL(add, one, two);
-    printf("add(%d, %d) = %d\n", read_nat(one), read_nat(two), read_nat(sum));
-    */
-
     void* fib = _$14(NULL, NULL);
     for (int i = 0; i < 8; ++i) {
         void* result = call(fib, make_nat(i));
         printf("fib(%d) = %d\n", i, read_nat(result));
     }
+    */
 
     return 0;
 }
