src/Extraction.v
@@ -175,6 +175,8 @@ Separate Extraction
 
    Oeuf.transf_to_cminor
    Oeuf.transf_to_asm
+   SourceLang.id_nat_reflect
+   SourceLang.long_id_reflect
    SourceLang.add_reflect
    SourceLang.fib_reflect
    Echo.initial_state_reflect
